A few improvements to the LinkedList module

test/LinkedList1.fst
@@ -4,6 +4,7 @@ module B = FStar.Buffer
 module HS = FStar.HyperStack
 module G = FStar.Ghost
 module L = FStar.List.Tot
+module U32 = FStar.UInt32
 
 open FStar.HyperStack.ST
 
@@ -24,7 +25,13 @@ and cell (a: Type0) =
       cell a
 
 /// Since linked lists go through a reference for indirection purposes, we
-/// enrich lists with a predicate that captures their length.
+/// enrich lists with a predicate that captures their length. This predicate
+/// will be needed for any traversal of the list, in order to show termination.
+/// Some points of interest:
+/// - the absence of cycles does not suffice to guarantee termination, as the
+///   number of references in the heap is potentially infinite;
+/// - the heap model allows us to select without showing liveness, which allows
+///   to de-couple the length predicate from the liveness predicate.
 let rec list_has_length #a (h: HS.mem) (c: t a) (l: nat):
   GTot bool (decreases l)
 =
@@ -36,17 +43,17 @@ let rec list_has_length #a (h: HS.mem) (c: t a) (l: nat):
       else
         list_has_length h next (l - 1)
 
-/// Note: a tempting solution might be to enrich the type of cells with an
-/// erased length that contains the "built-in" existentially quantified,
-/// proof-only, computationally-irrelevant length. This would, in turn,
-/// guarantee erasure by KreMLin and we would recover the type of linked lists
-/// that we hope for. This is tedious in practice, as the normalizer does not
-/// reduce underneath an `erased t`, leading to considerable type-checking
-/// difficulties.
+/// Note: all the ghost predicates and functions operate on a length of type
+/// nat; the Ghost effect guarantees that the length can only be used at
+/// run-time. Functions called at run-time will, conversely, use a length of
+/// type `erased nat`, which states that the length is
+/// computationally-irrelevant and can be safely removed from the resulting C
+/// code via a combination of F* + KreMLin erasure.
 
-/// This lemma ensures that when matching on a Cons cell, then recursively
-/// calling something on length (l - 1), we get automatically that (l - 1) is
-/// nat.
+/// When traversing a list `l` such that `list_has_length h l n`, it is often
+/// the case that we recursively visit the Cons cell, passing `n - 1` for the
+/// recursive call. This lemma ensures that Z3 can show that `n - 1` has type
+/// `nat`.
 let cons_nonzero_length #a (h: HS.mem) (c: ref (cell a)) (l: nat):
   Lemma
     (requires (list_has_length h c l /\ Cons? (HS.sel h c)))
@@ -54,6 +61,8 @@ let cons_nonzero_length #a (h: HS.mem) (c: ref (cell a)) (l: nat):
     [ SMTPat (list_has_length h c l); SMTPat (Cons? (HS.sel h c)) ] =
     ()
 
+/// The contraposition of this lemma allows deriving that if two lengths are
+/// different, then the corresponding references are disjoint.
 let rec length_injective #a (h: HS.mem) (c: ref (cell a)) (l1 l2: nat):
   Lemma
     (requires (list_has_length h c l1 /\ list_has_length h c l2))
@@ -66,9 +75,16 @@ let rec length_injective #a (h: HS.mem) (c: ref (cell a)) (l1 l2: nat):
       // Without `cons_nonzero_length`, we would need assert (l1 <> 0)
       length_injective h next (l1 - 1) (l2 - 1)
 
-/// A predicate that states that a single reference (the cell) is live.
-/// TODO: figure out why the predicate is called contains instead of live
-/// TODO: figure out why we need frameOf (see note to Aseem)
+/// For this example, we let all references live in the general region of the
+/// heap. The `contains` predicate is needed by several lemmas from the heap
+/// library, so we list it here.
+///
+/// The liveness predicate is `contains`: as an approximation, the underlying
+/// heap model represents each region as a map from addresses to their values,
+/// and contains asserts that the reference is in the domain of the map.
+///
+/// TODO: figure out why the predicate is called contains instead of
+/// TODO: figure out why we need frameOf
 let cell_is_live #a (h: HS.mem) (c: t a) =
   HS.frameOf c = HS.root /\
   HS.contains h c
@@ -102,14 +118,15 @@ let live #a (h: HS.mem) (l: t a) =
 /// As we start proving some degree of functional correctness, we will have to
 /// reason about non-interference, and state that some operations do not modify
 /// the footprint of a given list.
-/// TODO: proper patterns for quantifiers!
+/// TODO: there's a non-replayable hint here
 #set-options "--max_ifuel 0 --max_fuel 1"
 val footprint: (#a: Type) -> (h: HS.mem) -> (l: t a) -> (n: nat) -> Ghost (list (ref (cell a)))
   (requires (well_formed h l n))
   (ensures (fun refs ->
     let n_refs = L.length refs in
     n_refs = n /\
-    (forall (i: nat). i < n ==> well_formed h (L.index refs (n - 1 - i)) (i + 1))))
+    (forall (i: nat). {:pattern (L.index refs i)}
+      i < n ==> well_formed h (L.index refs i) (n - i))))
   (decreases n)
 
 let rec footprint #a h l n =
@@ -121,11 +138,18 @@ let rec footprint #a h l n =
       l :: refs
 #reset-options
 
+/// There are several views of references; by default, references do not support
+/// decidable equality, i.e. the heap model does not expose pointer comparisons.
+/// One can, however, reason about equality of addresses (ghostly, i.e. in
+/// proofs only) by using `HS.as_addr`. From two references having distinct
+/// addresses, it follows that writing to one leaves the other untouched.
+
 /// All the reasoning about the pop operation is done in this lemma. If `head`
 /// is not found in the footprint of `l`, then the specific write we perform for
 /// pop (we could be more generic!) leaves the two essential predicates
 /// untouched for l.
 /// TODO: this proof is slow / investigate
+
 val pop_preserves_live: (#a: Type) -> (h0: HS.mem) -> (head: ref (cell a)) -> (l: t a) -> (n: nat) ->
   Lemma
     (requires (
@@ -133,15 +157,16 @@ val pop_preserves_live: (#a: Type) -> (h0: HS.mem) -> (head: ref (cell a)) -> (l
       Cons? (HS.sel h0 head) /\
       well_formed h0 l n /\ (
       let refs = footprint h0 l n in
-      forall (i: nat). i < n ==> HS.as_addr head <> HS.as_addr (L.index refs i)
-    )))
+      forall (i: nat). // {:pattern well_formed h0 (L.index refs i) (n - i)}
+        i < n ==> HS.as_addr head <> HS.as_addr (L.index refs i))
+    ))
     (ensures (
       live h0 head /\
       Cons? (HS.sel h0 head) /\ (
       let next = Cons?.next (HS.sel h0 head) in
       let h1 = HS.upd h0 head (HS.sel h0 next) in
-      well_formed h1 l n
-    )))
+      well_formed h1 l n)
+    ))
     (decreases n)
     [ SMTPat (well_formed #a h0 l n); SMTPat (Cons? (HS.sel h0 head)) ]
 
@@ -152,16 +177,27 @@ let rec pop_preserves_live #a h0 head l n =
   | Cons l' _ ->
       pop_preserves_live h0 head l' (n - 1)
 
-/// Finally, the pop operation. The code is straightforward and crucially relies
-/// on the call to the lemma above. Note that at this stage we do not prove full
-/// functional correctness of our implementation. Rather, we just state that the
-/// lengths is as expected.
-/// TODO: move this code to use an erased integer... but merely computing n - 1
-/// below behind an erased type is tedious.
-val pop: (#a: Type) -> (#n: nat) -> (l: t a) ->
-  ST (option a)
-  (requires (fun h -> well_formed h l n))
+/// Finally, the pop operation. Our representation of linked lists is slightly
+/// unusual, owing to the fact that we do not have null references, and
+/// therefore represent the empty list as a reference to `Nil`. This means that
+/// popping an element off the front of the list can be done by merely writing
+/// the next cell in that reference. This is in contrast to the classic
+/// representation using null pointers, which requires the client to pass a
+/// pointer to a pointer, which is then filled with the address of the next
+/// cell, or null if this was the last element in the list.
+
+/// The code is straightforward and crucially relies on the call to the lemma
+/// above. Note that at this stage we do not prove full functional correctness
+/// of our implementation. Rather, we just state that the lengths is as
+/// expected.
+
+/// This version uses an erased integer n; we have to work a little bit to
+/// hide/reveal the computationally-irrelevant length.
+val pop: (#a: Type) -> (#n: G.erased nat) -> (l: t a) ->
+  Stack (option a)
+  (requires (fun h -> well_formed h l (G.reveal n)))
   (ensures (fun h0 v h1 ->
+    let n = G.reveal n in
     match v with
     | None -> n = 0 /\ well_formed h1 l n
     | Some _ -> n > 0 /\ well_formed h1 l (n - 1)
@@ -173,16 +209,60 @@ let pop #a #n l =
   | Cons next data ->
       let h0 = get () in
       l := !next;
-      pop_preserves_live #a h0 l next (n - 1);
+      pop_preserves_live #a h0 l next (G.reveal n - 1);
       Some data
 
-/// Purely a test function to see some actual code.
-let test_pop #n (l: t UInt32.t): ST UInt32.t
-  (requires (fun h -> well_formed h l n))
-  (ensures (fun _ _ _ -> true)) =
-  match pop #UInt32.t #n l with
-  | None -> 0ul
-  | Some x -> x
+val push: (#a: Type) -> (#n: G.erased nat) -> (l: t a) -> (x: a) ->
+  ST unit
+    (requires (fun h -> well_formed h l (G.reveal n)))
+    (ensures (fun h0 () h1 -> well_formed h1 l (G.reveal n + 1)))
+
+let push #a #n l x =
+  let c: ref (cell a) = ralloc HS.root !l in
+  // need to write a lemma that states that allocation preserves the live
+  // predicate for lists
+  l := Cons c x;
+  admit ()
+
+
+/// Connecting our predicate `list_has_length` to the regular length function.
+/// Note that this function takes a list whose length is unknown statically,
+/// because of the existential quantification.
+/// TODO: figure out why the `assert` is needed.
+val length (#a: Type) (gn: G.erased nat) (l: t a): Stack UInt32.t
+  (requires (fun h -> well_formed h l (G.reveal gn)))
+  (ensures (fun h0 n h1 ->
+    h0 == h1 /\
+    U32.v n = G.reveal gn
+  ))
+
+/// Note that we could have as easily returned an option, but sometimes fatal
+/// errors are just easier to handle for client code. The `C.String` module
+/// provides facilities for dealing with constant C string literals. It reveals
+/// that they are zero-terminated and allows looping over them if one wants to,
+/// say, copy an immutable constant string into a mutable buffer.
+let rec length #a gn l =
+  match !l with
+  | Nil ->
+      let h = get () in
+      assert (list_has_length h l 0);
+      0ul
+  | Cons next _ ->
+      let open U32 in
+      let h = get () in
+      let n = length (G.hide (G.reveal gn - 1)) next in
+      if n = 0xfffffffful then begin
+        C.String.(print !$"Integer overflow while computing length");
+        C.exit 255l;
+        0ul
+      end else
+        n +^ 1ul
   
+val main: unit -> ST (Int32.t) (fun _ -> true) (fun _ _ _ -> true)
 let main () =
-  0l
+  let l: ref (cell Int32.t) = ralloc HS.root Nil in
+  push #Int32.t #(G.hide 0) l 1l;
+  push #Int32.t #(G.hide 1) l 0l;
+  match pop #Int32.t #(G.hide 2) l with
+  | None -> 1l
+  | Some x -> x
